[Parikh] documentation for Parikh_Img.thy

Parikh/Parikh_Img.thy
@@ -1,3 +1,5 @@
+section \<open>Parikh images\<close>
+
 theory Parikh_Img
   imports 
     "Reg_Lang_Exp"
@@ -5,147 +7,144 @@ theory Parikh_Img
 begin
 
 
-section \<open>Parikh image\<close>
+subsection \<open>Definition and basic lemmas\<close>
 
-(* a Parikh vector is represented as a multiset *)
+text \<open>The Parikh vector of a finite word describes how often each symbol of the alphabet occurs in the word.
+We represent parikh vectors by multisets. The Parikh image of a language \<open>L\<close>, denoted by \<open>\<Psi> L\<close>,
+is then the set of Parikh vectors of all words in the language.\<close>
 
-(* compute Parikh vector for given word *)
 abbreviation parikh_vec where
   "parikh_vec \<equiv> mset"
 
-(* Parikh image for a given language *)
 definition parikh_img :: "'a lang \<Rightarrow> 'a multiset set" ("\<Psi>") where
-  "parikh_img L \<equiv> parikh_vec ` L"
+  "\<Psi> L \<equiv> parikh_vec ` L"
 
-
-(* TODO: really necessary? *)
-definition subseteq_comm :: "'t lang \<Rightarrow> 't lang \<Rightarrow> bool" where
-  "subseteq_comm L1 L2 \<equiv> \<Psi> L1 \<subseteq> \<Psi> L2"
-
-
-lemma parikh_img_Un [simp]: "parikh_img (L1 \<union> L2) = parikh_img L1 \<union> parikh_img L2"
+lemma parikh_img_Un [simp]: "\<Psi> (L1 \<union> L2) = \<Psi> L1 \<union> \<Psi> L2"
   by (auto simp add: parikh_img_def)
 
-lemma parikh_img_UNION: "parikh_img (\<Union>(L ` I)) = \<Union> ((\<lambda>i. parikh_img (L i)) ` I)"
+lemma parikh_img_UNION: "\<Psi> (\<Union>(L ` I)) = \<Union> ((\<lambda>i. \<Psi> (L i)) ` I)"
   by (auto simp add: parikh_img_def)
 
-lemma parikh_img_mono: "A \<subseteq> B \<Longrightarrow> parikh_img A \<subseteq> parikh_img B"
-  unfolding parikh_img_def by fast
-
-lemma parikh_img_mono_eq: "A = B \<Longrightarrow> parikh_img A = parikh_img B"
-  using parikh_img_mono by blast
-
-
-lemma parikh_img_Star_pow: "m \<in> parikh_img (eval (Star f) v) \<Longrightarrow> \<exists>n. m \<in> parikh_img (eval f v ^^ n)"
+lemma parikh_img_Star_pow: "m \<in> \<Psi> (eval (Star f) v) \<Longrightarrow> \<exists>n. m \<in> \<Psi> (eval f v ^^ n)"
 proof -
-  assume "m \<in> parikh_img (eval (rlexp.Star f) v)"
-  then have "m \<in> parikh_img (star (eval f v))" by simp
+  assume "m \<in> \<Psi> (eval (rlexp.Star f) v)"
+  then have "m \<in> \<Psi> (star (eval f v))" by simp
   then show ?thesis unfolding star_def by (simp add: parikh_img_UNION)
 qed
 
-
-lemma parikh_img_conc: "parikh_img (L1 @@ L2) = { m1 + m2 | m1 m2. m1 \<in> parikh_img L1 \<and> m2 \<in> parikh_img L2 }"
+lemma parikh_img_conc: "\<Psi> (L1 @@ L2) = { m1 + m2 | m1 m2. m1 \<in> \<Psi> L1 \<and> m2 \<in> \<Psi> L2 }"
   unfolding parikh_img_def by force
 
-lemma parikh_img_commut: "parikh_img (L1 @@ L2) = parikh_img (L2 @@ L1)"
+lemma parikh_img_commut: "\<Psi> (L1 @@ L2) = \<Psi> (L2 @@ L1)"
 proof -
-  have "{ m1 + m2 | m1 m2. m1 \<in> parikh_img L1 \<and> m2 \<in> parikh_img L2 } = 
-        { m2 + m1 | m1 m2. m1 \<in> parikh_img L1 \<and> m2 \<in> parikh_img L2 }"
+  have "{ m1 + m2 | m1 m2. m1 \<in> \<Psi> L1 \<and> m2 \<in> \<Psi> L2 } = 
+        { m2 + m1 | m1 m2. m1 \<in> \<Psi> L1 \<and> m2 \<in> \<Psi> L2 }"
     using add.commute by blast
   then show ?thesis
     using parikh_img_conc[of L1] parikh_img_conc[of L2] by auto
 qed
 
 
-lemma parikh_conc_right_subset: "parikh_img A \<subseteq> parikh_img B \<Longrightarrow> parikh_img (A @@ C) \<subseteq> parikh_img (B @@ C)"
+subsection \<open>Monotonicity properties\<close>
+
+lemma parikh_img_mono: "A \<subseteq> B \<Longrightarrow> \<Psi> A \<subseteq> \<Psi> B"
+  unfolding parikh_img_def by fast
+
+lemma parikh_img_mono_eq: "A = B \<Longrightarrow> \<Psi> A = \<Psi> B"
+  using parikh_img_mono by blast
+
+lemma parikh_conc_right_subset: "\<Psi> A \<subseteq> \<Psi> B \<Longrightarrow> \<Psi> (A @@ C) \<subseteq> \<Psi> (B @@ C)"
   by (auto simp add: parikh_img_conc)
 
-lemma parikh_conc_left_subset: "parikh_img A \<subseteq> parikh_img B \<Longrightarrow> parikh_img (C @@ A) \<subseteq> parikh_img (C @@ B)"
+lemma parikh_conc_left_subset: "\<Psi> A \<subseteq> \<Psi> B \<Longrightarrow> \<Psi> (C @@ A) \<subseteq> \<Psi> (C @@ B)"
   by (auto simp add: parikh_img_conc)
 
 lemma parikh_conc_subset:
-  assumes "parikh_img A \<subseteq> parikh_img C"
-      and "parikh_img B \<subseteq> parikh_img D"
-    shows "parikh_img (A @@ B) \<subseteq> parikh_img (C @@ D)"
+  assumes "\<Psi> A \<subseteq> \<Psi> C"
+      and "\<Psi> B \<subseteq> \<Psi> D"
+    shows "\<Psi> (A @@ B) \<subseteq> \<Psi> (C @@ D)"
   using assms parikh_conc_right_subset parikh_conc_left_subset by blast
 
-lemma parikh_conc_right: "parikh_img A = parikh_img B \<Longrightarrow> parikh_img (A @@ C) = parikh_img (B @@ C)"
+lemma parikh_conc_right: "\<Psi> A = \<Psi> B \<Longrightarrow> \<Psi> (A @@ C) = \<Psi> (B @@ C)"
   by (auto simp add: parikh_img_conc)
 
-lemma parikh_conc_left: "parikh_img A = parikh_img B \<Longrightarrow> parikh_img (C @@ A) = parikh_img (C @@ B)"
+lemma parikh_conc_left: "\<Psi> A = \<Psi> B \<Longrightarrow> \<Psi> (C @@ A) = \<Psi> (C @@ B)"
   by (auto simp add: parikh_img_conc)
 
-lemma parikh_pow_mono: "parikh_img A \<subseteq> parikh_img B \<Longrightarrow> parikh_img (A ^^ n) \<subseteq> parikh_img (B ^^ n)"
+lemma parikh_pow_mono: "\<Psi> A \<subseteq> \<Psi> B \<Longrightarrow> \<Psi> (A ^^ n) \<subseteq> \<Psi> (B ^^ n)"
   by (induction n) (auto simp add: parikh_img_conc)
 
+
 lemma parikh_star_mono:
-  assumes "parikh_img A \<subseteq> parikh_img B"
-  shows "parikh_img (star A) \<subseteq> parikh_img (star B)"
+  assumes "\<Psi> A \<subseteq> \<Psi> B"
+  shows "\<Psi> (star A) \<subseteq> \<Psi> (star B)"
 proof
   fix v
-  assume "v \<in> parikh_img (star A)"
+  assume "v \<in> \<Psi> (star A)"
   then obtain w where w_intro: "parikh_vec w = v \<and> w \<in> star A" unfolding parikh_img_def by blast
   then obtain n where "w \<in> A ^^ n" unfolding star_def by blast
-  then have "v \<in> parikh_img (A ^^ n)" using w_intro unfolding parikh_img_def by blast
-  with assms have "v \<in> parikh_img (B ^^ n)" using parikh_pow_mono by blast
-  then show "v \<in> parikh_img (star B)" unfolding star_def using parikh_img_UNION by fastforce
+  then have "v \<in> \<Psi> (A ^^ n)" using w_intro unfolding parikh_img_def by blast
+  with assms have "v \<in> \<Psi> (B ^^ n)" using parikh_pow_mono by blast
+  then show "v \<in> \<Psi> (star B)" unfolding star_def using parikh_img_UNION by fastforce
 qed
 
 lemma parikh_star_mono_eq:
-  assumes "parikh_img A = parikh_img B"
-  shows "parikh_img (star A) = parikh_img (star B)"
+  assumes "\<Psi> A = \<Psi> B"
+  shows "\<Psi> (star A) = \<Psi> (star B)"
   using parikh_star_mono by (metis Orderings.order_eq_iff assms)
 
 
 lemma parikh_img_subst_mono:
-  assumes "\<forall>i. parikh_img (eval (A i) v) \<subseteq> parikh_img (eval (B i) v)"
-  shows "parikh_img (eval (subst A f) v) \<subseteq> parikh_img (eval (subst B f) v)"
+  assumes "\<forall>i. \<Psi> (eval (A i) v) \<subseteq> \<Psi> (eval (B i) v)"
+  shows "\<Psi> (eval (subst A f) v) \<subseteq> \<Psi> (eval (subst B f) v)"
 using assms proof (induction f)
   case (Concat f1 f2)
-  then have "parikh_img (eval (subst A f1) v @@ eval (subst A f2) v)
-              \<subseteq> parikh_img (eval (subst B f1) v @@ eval (subst B f2) v)"
+  then have "\<Psi> (eval (subst A f1) v @@ eval (subst A f2) v)
+              \<subseteq> \<Psi> (eval (subst B f1) v @@ eval (subst B f2) v)"
     using parikh_conc_subset by blast
   then show ?case by simp
 next
   case (Star f)
-  then have "parikh_img (star (eval (subst A f) v)) \<subseteq> parikh_img (star (eval (subst B f) v))"
+  then have "\<Psi> (star (eval (subst A f) v)) \<subseteq> \<Psi> (star (eval (subst B f) v))"
     using parikh_star_mono by blast
   then show ?case by simp
 qed auto
 
 lemma parikh_img_subst_mono_upd:
-  assumes "parikh_img (eval A v) \<subseteq> parikh_img (eval B v)"
-  shows "parikh_img (eval (subst (Var(x := A)) f) v) \<subseteq> parikh_img (eval (subst (Var(x := B)) f) v)"
+  assumes "\<Psi> (eval A v) \<subseteq> \<Psi> (eval B v)"
+  shows "\<Psi> (eval (subst (Var(x := A)) f) v) \<subseteq> \<Psi> (eval (subst (Var(x := B)) f) v)"
   using parikh_img_subst_mono[of "Var(x := A)" v "Var(x := B)"] assms by auto
 
 lemma parikh_img_subst_mono_eq:
-  assumes "\<forall>i. parikh_img (eval (A i) v) = parikh_img (eval (B i) v)"
-  shows "parikh_img (eval (subst (\<lambda>i. A i) f) v) = parikh_img (eval (subst (\<lambda>i. B i) f) v)"
+  assumes "\<forall>i. \<Psi> (eval (A i) v) = \<Psi> (eval (B i) v)"
+  shows "\<Psi> (eval (subst (\<lambda>i. A i) f) v) = \<Psi> (eval (subst (\<lambda>i. B i) f) v)"
   using parikh_img_subst_mono assms by blast
 
+
 lemma rlexp_mono_parikh:
-  assumes "\<forall>i \<in> vars f. parikh_img (v i) \<subseteq> parikh_img (v' i)"
-  shows "parikh_img (eval f v) \<subseteq> parikh_img (eval f v')"
+  assumes "\<forall>i \<in> vars f. \<Psi> (v i) \<subseteq> \<Psi> (v' i)"
+  shows "\<Psi> (eval f v) \<subseteq> \<Psi> (eval f v')"
 using assms proof (induction rule: rlexp.induct)
 case (Concat f1 f2)
-  then have "parikh_img (eval f1 v @@ eval f2 v) \<subseteq> parikh_img (eval f1 v' @@ eval f2 v')"
+  then have "\<Psi> (eval f1 v @@ eval f2 v) \<subseteq> \<Psi> (eval f1 v' @@ eval f2 v')"
     using parikh_conc_subset by (metis UnCI vars.simps(4))
   then show ?case by simp
 qed (auto simp add: SUP_mono' parikh_img_UNION parikh_star_mono)
 
-
 lemma rlexp_mono_parikh_eq:
-  assumes "\<forall>i \<in> vars f. parikh_img (v i) = parikh_img (v' i)"
-  shows "parikh_img (eval f v) = parikh_img (eval f v')"
+  assumes "\<forall>i \<in> vars f. \<Psi> (v i) = \<Psi> (v' i)"
+  shows "\<Psi> (eval f v) = \<Psi> (eval f v')"
   using assms rlexp_mono_parikh by blast
 
 
 
-section \<open>(E\<union>F)* and E*F* have the same Parikh image\<close>
+subsection \<open>\<^latex>\<open>$\Psi \; (A \cup B)^* = \Psi \; A^* B^*$\<close>\<close>
+
+text \<open>This property is claimed by Pilling in (TODO: citation) and will be needed in the rest of the proof.\<close>
 
 lemma parikh_img_union_pow_aux1:
-  assumes "v \<in> parikh_img ((A \<union> B) ^^ n)"
-    shows "v \<in> parikh_img (\<Union>i \<le> n. A ^^ i @@ B ^^ (n-i))"
+  assumes "v \<in> \<Psi> ((A \<union> B) ^^ n)"
+    shows "v \<in> \<Psi> (\<Union>i \<le> n. A ^^ i @@ B ^^ (n-i))"
 using assms proof (induction n arbitrary: v)
   case 0
   then show ?case by simp
@@ -156,28 +155,28 @@ next
   then obtain w1 w2 where w1_w2_intro: "w = w1@w2 \<and> w1 \<in> A \<union> B \<and> w2 \<in> (A \<union> B) ^^ n" by fastforce
   let ?v1 = "parikh_vec w1" and ?v2 = "parikh_vec w2"
 
-  from w1_w2_intro have "?v2 \<in> parikh_img ((A \<union> B) ^^ n)" unfolding parikh_img_def by blast
-  with Suc.IH have "?v2 \<in> parikh_img (\<Union>i \<le> n. A ^^ i @@ B ^^ (n-i))" by auto
+  from w1_w2_intro have "?v2 \<in> \<Psi> ((A \<union> B) ^^ n)" unfolding parikh_img_def by blast
+  with Suc.IH have "?v2 \<in> \<Psi> (\<Union>i \<le> n. A ^^ i @@ B ^^ (n-i))" by auto
   then obtain w2' where w2'_intro: "parikh_vec w2' = parikh_vec w2 \<and>
       w2' \<in> (\<Union>i \<le> n. A ^^ i @@ B ^^ (n-i))" unfolding parikh_img_def by fastforce
   then obtain i where i_intro: "i \<le> n \<and> w2' \<in> A ^^ i @@ B ^^ (n-i)" by blast
 
   from w1_w2_intro w2'_intro have "parikh_vec w = parikh_vec (w1@w2')"
     by simp
-  moreover have "parikh_vec (w1@w2') \<in> parikh_img (\<Union>i \<le> Suc n. A ^^ i @@ B ^^ (Suc n-i))"
+  moreover have "parikh_vec (w1@w2') \<in> \<Psi> (\<Union>i \<le> Suc n. A ^^ i @@ B ^^ (Suc n-i))"
   proof (cases "w1 \<in> A")
     case True
     with i_intro have Suc_i_valid: "Suc i \<le> Suc n" and "w1@w2' \<in> A ^^ (Suc i) @@ B ^^ (Suc n - Suc i)"
       by (auto simp add: conc_assoc)
-    then have "parikh_vec (w1@w2') \<in> parikh_img (A ^^ (Suc i) @@ B ^^ (Suc n - Suc i))"
+    then have "parikh_vec (w1@w2') \<in> \<Psi> (A ^^ (Suc i) @@ B ^^ (Suc n - Suc i))"
       unfolding parikh_img_def by blast
     with Suc_i_valid parikh_img_UNION show ?thesis by fast
   next
     case False
     with w1_w2_intro have "w1 \<in> B" by blast
-    with i_intro have "parikh_vec (w1@w2') \<in> parikh_img (B @@ A ^^ i @@ B ^^ (n-i))"
+    with i_intro have "parikh_vec (w1@w2') \<in> \<Psi> (B @@ A ^^ i @@ B ^^ (n-i))"
       unfolding parikh_img_def by blast
-    then have "parikh_vec (w1@w2') \<in> parikh_img (A ^^ i @@ B ^^ (Suc n-i))"
+    then have "parikh_vec (w1@w2') \<in> \<Psi> (A ^^ i @@ B ^^ (Suc n-i))"
       using parikh_img_commut conc_assoc
       by (metis Suc_diff_le conc_pow_comm i_intro lang_pow.simps(2))
     with i_intro parikh_img_UNION show ?thesis by fastforce
@@ -187,16 +186,16 @@ qed
 
 
 lemma parikh_img_star_aux1:
-  assumes "v \<in> parikh_img (star (A \<union> B))"
-  shows "v \<in> parikh_img (star A @@ star B)"
+  assumes "v \<in> \<Psi> (star (A \<union> B))"
+  shows "v \<in> \<Psi> (star A @@ star B)"
 proof -
-  from assms have "v \<in> (\<Union>n. parikh_img ((A \<union> B) ^^ n))"
+  from assms have "v \<in> (\<Union>n. \<Psi> ((A \<union> B) ^^ n))"
     unfolding star_def using parikh_img_UNION by metis
-  then obtain n where "v \<in> parikh_img ((A \<union> B) ^^ n)" by blast
-  then have "v \<in> parikh_img (\<Union>i \<le> n. A ^^ i @@ B ^^ (n-i))"
+  then obtain n where "v \<in> \<Psi> ((A \<union> B) ^^ n)" by blast
+  then have "v \<in> \<Psi> (\<Union>i \<le> n. A ^^ i @@ B ^^ (n-i))"
     using parikh_img_union_pow_aux1 by auto
-  then have "v \<in> (\<Union>i\<le>n. parikh_img (A ^^ i @@ B ^^ (n-i)))" using parikh_img_UNION by metis
-  then obtain i where "i\<le>n \<and> v \<in> parikh_img (A ^^ i @@ B ^^ (n-i))" by blast
+  then have "v \<in> (\<Union>i\<le>n. \<Psi> (A ^^ i @@ B ^^ (n-i)))" using parikh_img_UNION by metis
+  then obtain i where "i\<le>n \<and> v \<in> \<Psi> (A ^^ i @@ B ^^ (n-i))" by blast
   then obtain w where w_intro: "parikh_vec w = v \<and> w \<in> A ^^ i @@ B ^^ (n-i)"
     unfolding parikh_img_def by blast
   then obtain w1 w2 where w_decomp: "w=w1@w2 \<and> w1 \<in> A ^^ i \<and> w2 \<in> B ^^ (n-i)" by blast
@@ -206,8 +205,8 @@ proof -
 qed
 
 lemma parikh_img_star_aux2:
-  assumes "v \<in> parikh_img (star A @@ star B)"
-  shows "v \<in> parikh_img (star (A \<union> B))"
+  assumes "v \<in> \<Psi> (star A @@ star B)"
+  shows "v \<in> \<Psi> (star (A \<union> B))"
 proof -
   from assms obtain w where w_intro: "parikh_vec w = v \<and> w \<in> star A @@ star B"
     unfolding parikh_img_def by blast
@@ -220,103 +219,106 @@ proof -
 qed
 
 
-lemma parikh_img_star: "parikh_img (star (A \<union> B)) = parikh_img (star A @@ star B)"
+lemma parikh_img_star: "\<Psi> (star (A \<union> B)) = \<Psi> (star A @@ star B)"
 proof
-  show "parikh_img (star (A \<union> B)) \<subseteq> parikh_img (star A @@ star B)" using parikh_img_star_aux1 by auto
-  show "parikh_img (star A @@ star B) \<subseteq> parikh_img (star (A \<union> B))" using parikh_img_star_aux2 by auto
+  show "\<Psi> (star (A \<union> B)) \<subseteq> \<Psi> (star A @@ star B)" using parikh_img_star_aux1 by auto
+  show "\<Psi> (star A @@ star B) \<subseteq> \<Psi> (star (A \<union> B))" using parikh_img_star_aux2 by auto
 qed
 
 
 
-section \<open>(E*F)* and {\<epsilon>} \<union> E*F*F have the same Parikh image\<close>
+subsection \<open>\<^latex>\<open>$\Psi \; (E^* F)^* = \Psi \; \left(\{\varepsilon\} \cup E^* F^* F\right)$\<close>\<close>
 
-(* It even holds = but this is not necessary *)
-lemma parikh_img_conc_pow: "parikh_img ((A @@ B) ^^ n) \<subseteq> parikh_img (A ^^ n @@ B ^^ n)"
+text \<open>This property (where \<^latex>\<open>$\varepsilon$\<close> denotes the empty word) is claimed by
+Pilling as well (TODO: citation); we will need it later.\<close>
+
+(* It even holds = but \<subseteq> suffices for the proof *)
+lemma parikh_img_conc_pow: "\<Psi> ((A @@ B) ^^ n) \<subseteq> \<Psi> (A ^^ n @@ B ^^ n)"
 proof (induction n)
   case (Suc n)
-  then have "parikh_img ((A @@ B) ^^ n @@ A @@ B) \<subseteq> parikh_img (A ^^ n @@ B ^^ n @@ A @@ B)"
+  then have "\<Psi> ((A @@ B) ^^ n @@ A @@ B) \<subseteq> \<Psi> (A ^^ n @@ B ^^ n @@ A @@ B)"
     using parikh_conc_right_subset conc_assoc by metis
-  also have "\<dots> = parikh_img (A ^^ n @@ A @@ B ^^ n @@ B)"
+  also have "\<dots> = \<Psi> (A ^^ n @@ A @@ B ^^ n @@ B)"
     by (metis parikh_img_commut conc_assoc parikh_conc_left)
   finally show ?case by (simp add: conc_assoc conc_pow_comm)
 qed simp
 
-lemma parikh_img_conc_star: "parikh_img (star (A @@ B)) \<subseteq> parikh_img (star A @@ star B)"
+lemma parikh_img_conc_star: "\<Psi> (star (A @@ B)) \<subseteq> \<Psi> (star A @@ star B)"
 proof
   fix v
-  assume "v \<in> parikh_img (star (A @@ B))"
-  then have "\<exists>n. v \<in> parikh_img ((A @@ B) ^^ n)" unfolding star_def by (simp add: parikh_img_UNION)
-  then obtain n where "v \<in> parikh_img ((A @@ B) ^^ n)" by blast
-  with parikh_img_conc_pow have "v \<in> parikh_img (A ^^ n @@ B ^^ n)" by fast
-  then have "v \<in> parikh_img (A ^^ n @@ star B)"
+  assume "v \<in> \<Psi> (star (A @@ B))"
+  then have "\<exists>n. v \<in> \<Psi> ((A @@ B) ^^ n)" unfolding star_def by (simp add: parikh_img_UNION)
+  then obtain n where "v \<in> \<Psi> ((A @@ B) ^^ n)" by blast
+  with parikh_img_conc_pow have "v \<in> \<Psi> (A ^^ n @@ B ^^ n)" by fast
+  then have "v \<in> \<Psi> (A ^^ n @@ star B)"
     unfolding star_def using parikh_conc_left_subset
     by (metis (no_types, lifting) Sup_upper parikh_img_mono rangeI subset_eq)
-  then show "v \<in> parikh_img (star A @@ star B)"
+  then show "v \<in> \<Psi> (star A @@ star B)"
     unfolding star_def using parikh_conc_right_subset
     by (metis (no_types, lifting) Sup_upper parikh_img_mono rangeI subset_eq)
 qed
 
-lemma parikh_img_conc_pow2: "parikh_img ((A @@ B) ^^ Suc n) \<subseteq> parikh_img (star A @@ star B @@ B)"
+lemma parikh_img_conc_pow2: "\<Psi> ((A @@ B) ^^ Suc n) \<subseteq> \<Psi> (star A @@ star B @@ B)"
 proof
   fix v
-  assume "v \<in> parikh_img ((A @@ B) ^^ Suc n)"
-  with parikh_img_conc_pow have "v \<in> parikh_img (A ^^ Suc n @@ B ^^ n @@ B)"
+  assume "v \<in> \<Psi> ((A @@ B) ^^ Suc n)"
+  with parikh_img_conc_pow have "v \<in> \<Psi> (A ^^ Suc n @@ B ^^ n @@ B)"
     by (metis conc_pow_comm lang_pow.simps(2) subsetD)
-  then have "v \<in> parikh_img (star A @@ B ^^ n @@ B)"
+  then have "v \<in> \<Psi> (star A @@ B ^^ n @@ B)"
     unfolding star_def using parikh_conc_right_subset
     by (metis (no_types, lifting) Sup_upper parikh_img_mono rangeI subset_eq)
-  then show "v \<in> parikh_img (star A @@ star B @@ B)"
+  then show "v \<in> \<Psi> (star A @@ star B @@ B)"
     unfolding star_def using parikh_conc_right_subset parikh_conc_left_subset
     by (metis (no_types, lifting) Sup_upper parikh_img_mono rangeI subset_eq)
 qed
 
 lemma parikh_img_star2_aux1:
-  "parikh_img (star (star E @@ F)) \<subseteq> parikh_img ({[]} \<union> star E @@ star F @@ F)"
+  "\<Psi> (star (star E @@ F)) \<subseteq> \<Psi> ({[]} \<union> star E @@ star F @@ F)"
 proof
   fix v
-  assume "v \<in> parikh_img (star (star E @@ F))"
-  then have "\<exists>n. v \<in> parikh_img ((star E @@ F) ^^ n)"
+  assume "v \<in> \<Psi> (star (star E @@ F))"
+  then have "\<exists>n. v \<in> \<Psi> ((star E @@ F) ^^ n)"
     unfolding star_def by (simp add: parikh_img_UNION)
-  then obtain n where v_in_pow_n: "v \<in> parikh_img ((star E @@ F) ^^ n)" by blast
-  show "v \<in> parikh_img ({[]} \<union> star E @@ star F @@ F)"
+  then obtain n where v_in_pow_n: "v \<in> \<Psi> ((star E @@ F) ^^ n)" by blast
+  show "v \<in> \<Psi> ({[]} \<union> star E @@ star F @@ F)"
   proof (cases n)
     case 0
     with v_in_pow_n have "v = parikh_vec []" unfolding parikh_img_def by simp
     then show ?thesis unfolding parikh_img_def by blast
   next
     case (Suc m)
-    with parikh_img_conc_pow2 v_in_pow_n have "v \<in> parikh_img (star (star E) @@ star F @@ F)" by blast
+    with parikh_img_conc_pow2 v_in_pow_n have "v \<in> \<Psi> (star (star E) @@ star F @@ F)" by blast
     then show ?thesis by (metis UnCI parikh_img_Un star_idemp)
   qed
 qed
 
-lemma parikh_img_star2_aux2: "parikh_img (star E @@ star F @@ F) \<subseteq> parikh_img (star (star E @@ F))"
+lemma parikh_img_star2_aux2: "\<Psi> (star E @@ star F @@ F) \<subseteq> \<Psi> (star (star E @@ F))"
 proof -
   have "F \<subseteq> star E @@ F" unfolding star_def using Nil_in_star
     by (metis concI_if_Nil1 star_def subsetI)
-  then have "parikh_img (star E @@ F @@ star F) \<subseteq> parikh_img (star E @@ F @@ star (star E @@ F))"
+  then have "\<Psi> (star E @@ F @@ star F) \<subseteq> \<Psi> (star E @@ F @@ star (star E @@ F))"
     using parikh_conc_left_subset parikh_img_mono parikh_star_mono by meson
-  also have "\<dots> \<subseteq> parikh_img (star (star E @@ F))"
+  also have "\<dots> \<subseteq> \<Psi> (star (star E @@ F))"
     by (metis conc_assoc inf_sup_ord(3) parikh_img_mono star_unfold_left)
   finally show ?thesis using conc_star_comm by metis
 qed
 
-lemma parikh_img_star2: "parikh_img (star (star E @@ F)) = parikh_img ({[]} \<union> star E @@ star F @@ F)"
+lemma parikh_img_star2: "\<Psi> (star (star E @@ F)) = \<Psi> ({[]} \<union> star E @@ star F @@ F)"
 proof
   from parikh_img_star2_aux1
-    show "parikh_img (star (star E @@ F)) \<subseteq> parikh_img ({[]} \<union> star E @@ star F @@ F)" .
+    show "\<Psi> (star (star E @@ F)) \<subseteq> \<Psi> ({[]} \<union> star E @@ star F @@ F)" .
   from parikh_img_star2_aux2
-    show "parikh_img ({[]} \<union> star E @@ star F @@ F) \<subseteq> parikh_img (star (star E @@ F))"
+    show "\<Psi> ({[]} \<union> star E @@ star F @@ F) \<subseteq> \<Psi> (star (star E @@ F))"
     by (metis le_sup_iff parikh_img_Un star_unfold_left sup.cobounded2)
 qed
 
 
 
-section \<open>A homogeneous-like property for regular functions\<close>
+subsection \<open>A homogeneous-like property for regular functions\<close>
 
 lemma rlexp_homogeneous_aux:
   assumes "v x = star Y @@ Z"
-    shows "parikh_img (eval f v) \<subseteq> parikh_img (star Y @@ eval f (v(x := Z)))"
+    shows "\<Psi> (eval f v) \<subseteq> \<Psi> (star Y @@ eval f (v(x := Z)))"
 using assms proof (induction f)
   case (Var y)
   show ?case
@@ -334,129 +336,116 @@ next
   then show ?case by (simp add: parikh_img_mono)
 next
   case (Union f g)
-  then have "parikh_img (eval (Union f g) v) \<subseteq> parikh_img (star Y @@ eval f (v(x := Z)) \<union>
+  then have "\<Psi> (eval (Union f g) v) \<subseteq> \<Psi> (star Y @@ eval f (v(x := Z)) \<union>
                                                             star Y @@ eval g (v(x := Z)))"
     by fastforce
   then show ?case by (metis conc_Un_distrib(1) eval.simps(3))
 next
   case (Concat f g)
-  then have "parikh_img (eval (Concat f g) v) \<subseteq> parikh_img ((star Y @@ eval f (v(x := Z)))
+  then have "\<Psi> (eval (Concat f g) v) \<subseteq> \<Psi> ((star Y @@ eval f (v(x := Z)))
                                                           @@ star Y @@ eval g (v(x := Z)))"
     by (metis eval.simps(4) parikh_conc_subset)
-  also have "\<dots> = parikh_img (star Y @@ star Y @@ eval f (v(x := Z)) @@ eval g (v(x := Z)))"
+  also have "\<dots> = \<Psi> (star Y @@ star Y @@ eval f (v(x := Z)) @@ eval g (v(x := Z)))"
     by (metis conc_assoc parikh_conc_right parikh_img_commut)
-  also have "\<dots> = parikh_img (star Y @@ eval f (v(x := Z)) @@ eval g (v(x := Z)))"
+  also have "\<dots> = \<Psi> (star Y @@ eval f (v(x := Z)) @@ eval g (v(x := Z)))"
     by (metis conc_assoc conc_star_star)
   finally show ?case by (metis eval.simps(4))
 next
   case (Star f)
-  then have "parikh_img (star (eval f v)) \<subseteq> parikh_img (star (star Y @@ eval f (v(x := Z))))"
+  then have "\<Psi> (star (eval f v)) \<subseteq> \<Psi> (star (star Y @@ eval f (v(x := Z))))"
     using parikh_star_mono by metis
-  also from parikh_img_conc_star have "\<dots> \<subseteq> parikh_img (star Y @@ star (eval f (v(x := Z))))"
+  also from parikh_img_conc_star have "\<dots> \<subseteq> \<Psi> (star Y @@ star (eval f (v(x := Z))))"
     by fastforce
   finally show ?case by (metis eval.simps(5))
 qed
 
-lemma rlexp_homogeneous:  "parikh_img (eval (subst (Var(x := Concat (Star y) z)) f) v)
-                          \<subseteq> parikh_img (eval (Concat (Star y) (subst (Var(x := z)) f)) v)"
-                          (is "parikh_img ?L \<subseteq> parikh_img ?R")
+text \<open>Now we can prove the desired homogeneous-like property which will become useful later:\<close>
+(* Pilling even claims =, but \<supseteq> does not hold in my opinion and \<subseteq> suffices for the remaining proof anyway *)
+lemma rlexp_homogeneous:  "\<Psi> (eval (subst (Var(x := Concat (Star y) z)) f) v)
+                          \<subseteq> \<Psi> (eval (Concat (Star y) (subst (Var(x := z)) f)) v)"
+                          (is "\<Psi> ?L \<subseteq> \<Psi> ?R")
 proof -
   let ?v' = "v(x := star (eval y v) @@ eval z v)"
-  have "parikh_img ?L = parikh_img (eval f ?v')" using substitution_lemma_update[where f=f] by simp
-  also have "\<dots> \<subseteq> parikh_img (star (eval y v) @@ eval f (?v'(x := eval z v)))"
+  have "\<Psi> ?L = \<Psi> (eval f ?v')" using substitution_lemma_update[where f=f] by simp
+  also have "\<dots> \<subseteq> \<Psi> (star (eval y v) @@ eval f (?v'(x := eval z v)))"
     using rlexp_homogeneous_aux[of ?v'] unfolding fun_upd_def by auto
-  also have "\<dots> = parikh_img ?R" using substitution_lemma[of "v(x := eval z v)"] by simp
-  finally show ?thesis .
-qed
-
-(* reformulate previous lemma with regular functions as arguments instead of languages *)
-lemma rlexp_homogeneous2:
-    shows "parikh_img (eval (subst (Var(x := Concat (Star y) z)) f) v)
-            \<subseteq> parikh_img (eval (Concat (Star y) (subst (Var(x := z)) f)) v)"
-            (is "parikh_img ?L \<subseteq> parikh_img ?R")
-proof -
-  let ?v' = "v(x := star (eval y v) @@ eval z v)"
-  have "parikh_img ?L = parikh_img (eval f ?v')"
-    using substitution_lemma[of ?v' "Var(x := Concat (Star y) z)"] by fastforce
-  also have "\<dots> \<subseteq> parikh_img (star (eval y v) @@ eval f (?v'(x := eval z v)))"
-    using rlexp_homogeneous_aux[of ?v'] by (meson fun_upd_apply)
-  also have "\<dots> = parikh_img ?R" using substitution_lemma[of "?v'(x := eval z v)"] by simp
+  also have "\<dots> = \<Psi> ?R" using substitution_lemma[of "v(x := eval z v)"] by simp
   finally show ?thesis .
 qed
 
 
-
-section \<open>Extension of Arden's lemma to Parikh images\<close>
+subsection \<open>Extension of Arden's lemma to Parikh images\<close>
 
 lemma parikh_img_arden_aux:
-  assumes "parikh_img (A @@ X \<union> B) \<subseteq> parikh_img X"
-  shows "parikh_img (A ^^ n @@ B) \<subseteq> parikh_img X"
+  assumes "\<Psi> (A @@ X \<union> B) \<subseteq> \<Psi> X"
+  shows "\<Psi> (A ^^ n @@ B) \<subseteq> \<Psi> X"
 using assms proof (induction n)
   case 0
   then show ?case by auto
 next
   case (Suc n)
-  then have "parikh_img (A ^^ (Suc n) @@ B) \<subseteq> parikh_img (A @@ A ^^ n @@B)"
+  then have "\<Psi> (A ^^ (Suc n) @@ B) \<subseteq> \<Psi> (A @@ A ^^ n @@B)"
     by (simp add: conc_assoc)
-  moreover from Suc parikh_conc_left have "\<dots> \<subseteq> parikh_img (A @@ X)"
+  moreover from Suc parikh_conc_left have "\<dots> \<subseteq> \<Psi> (A @@ X)"
     by (metis conc_Un_distrib(1) parikh_img_Un sup.orderE sup.orderI)
-  moreover from Suc.prems have "\<dots> \<subseteq> parikh_img X" by auto
+  moreover from Suc.prems have "\<dots> \<subseteq> \<Psi> X" by auto
   ultimately show ?case by fast
 qed
 
 lemma parikh_img_arden:
-  assumes "parikh_img (A @@ X \<union> B) \<subseteq> parikh_img X"
-  shows "parikh_img (star A @@ B) \<subseteq> parikh_img X"
+  assumes "\<Psi> (A @@ X \<union> B) \<subseteq> \<Psi> X"
+  shows "\<Psi> (star A @@ B) \<subseteq> \<Psi> X"
 proof
   fix x
-  assume "x \<in> parikh_img (star A @@ B)"
-  then have "\<exists>n. x \<in> parikh_img (A ^^ n @@ B)"
+  assume "x \<in> \<Psi> (star A @@ B)"
+  then have "\<exists>n. x \<in> \<Psi> (A ^^ n @@ B)"
     unfolding star_def by (simp add: conc_UNION_distrib(2) parikh_img_UNION)
-  then obtain n where "x \<in> parikh_img (A ^^ n @@ B)" by blast
-  then show "x \<in> parikh_img X" using parikh_img_arden_aux[OF assms] by fast
+  then obtain n where "x \<in> \<Psi> (A ^^ n @@ B)" by blast
+  then show "x \<in> \<Psi> X" using parikh_img_arden_aux[OF assms] by fast
 qed
 
 
-section \<open>Equivalence class of languages with same Parikh image\<close>
+subsection \<open>Equivalence class of languages with identical Parikh image\<close>
+
+text \<open>For a given language \<open>L\<close>, we define the equivalence class of all languages with identical Parikh
+image:\<close>
 
 definition parikh_img_eq_class :: "'a lang \<Rightarrow> 'a lang set" where
-  "parikh_img_eq_class L \<equiv> {L'. parikh_img L' = parikh_img L}"
+  "parikh_img_eq_class L \<equiv> {L'. \<Psi> L' = \<Psi> L}"
 
-
-lemma parikh_img_Union_class: "parikh_img A = parikh_img (\<Union>(parikh_img_eq_class A))"
+lemma parikh_img_Union_class: "\<Psi> A = \<Psi> (\<Union>(parikh_img_eq_class A))"
 proof
   let ?A' = "\<Union>(parikh_img_eq_class A)"
-  show "parikh_img A \<subseteq> parikh_img ?A'"
+  show "\<Psi> A \<subseteq> \<Psi> ?A'"
     unfolding parikh_img_eq_class_def by (simp add: Union_upper parikh_img_mono)
 
-  show "parikh_img ?A' \<subseteq> parikh_img A"
+  show "\<Psi> ?A' \<subseteq> \<Psi> A"
   proof
     fix v
-    assume "v \<in> parikh_img ?A'"
+    assume "v \<in> \<Psi> ?A'"
     then obtain a where a_intro: "parikh_vec a = v \<and> a \<in> ?A'"
       unfolding parikh_img_def by blast
     then obtain L where L_intro: "a \<in> L \<and> L \<in> parikh_img_eq_class A"
       unfolding parikh_img_eq_class_def by blast
-    then have "parikh_img L = parikh_img A" unfolding parikh_img_eq_class_def by fastforce
-    with a_intro L_intro show "v \<in> parikh_img A" unfolding parikh_img_def by blast
+    then have "\<Psi> L = \<Psi> A" unfolding parikh_img_eq_class_def by fastforce
+    with a_intro L_intro show "v \<in> \<Psi> A" unfolding parikh_img_def by blast
   qed
 qed
 
-
 lemma subseteq_comm_subseteq:
-  assumes "parikh_img A \<subseteq> parikh_img B"
+  assumes "\<Psi> A \<subseteq> \<Psi> B"
   shows "A \<subseteq> \<Union>(parikh_img_eq_class B)" (is "A \<subseteq> ?B'")
 proof
   fix a
   assume a_in_A: "a \<in> A"
-  from assms have "parikh_img A \<subseteq> parikh_img ?B'"
+  from assms have "\<Psi> A \<subseteq> \<Psi> ?B'"
     using parikh_img_Union_class by blast
-  with a_in_A have vec_a_in_B': "parikh_vec a \<in> parikh_img ?B'" unfolding parikh_img_def by fast
+  with a_in_A have vec_a_in_B': "parikh_vec a \<in> \<Psi> ?B'" unfolding parikh_img_def by fast
   then have "\<exists>b. parikh_vec b = parikh_vec a \<and> b \<in> ?B'"
     unfolding parikh_img_def by fastforce
   then obtain b where b_intro: "parikh_vec b = parikh_vec a \<and> b \<in> ?B'" by blast
-  with vec_a_in_B' have "parikh_img (?B' \<union> {a}) = parikh_img ?B'"unfolding parikh_img_def by blast
-  with parikh_img_Union_class have "parikh_img (?B' \<union> {a}) = parikh_img B" by blast
+  with vec_a_in_B' have "\<Psi> (?B' \<union> {a}) = \<Psi> ?B'"unfolding parikh_img_def by blast
+  with parikh_img_Union_class have "\<Psi> (?B' \<union> {a}) = \<Psi> B" by blast
   then show "a \<in> ?B'" unfolding parikh_img_eq_class_def by blast
 qed
 
